proof/crefine/RISCV64/SchedContext_C.thy
@@ -11,25 +11,657 @@ begin
 
 context kernel_m begin
 
+lemma refill_next_ccorres:
+  "ccorres (\<lambda>next next'. next = unat next') ret__unsigned_long_'
+     (active_sc_at' scPtr and invs' and K (Suc idx < 2 ^ word_bits))
+     (\<lbrace>\<acute>sc = Ptr scPtr\<rbrace> \<inter> \<lbrace>\<acute>index = word_of_nat idx\<rbrace>) []
+     (getRefillNext scPtr idx) (Call refill_next_'proc)"
+  supply len_bit0[simp del]
+  apply (cinit lift: sc_' index_'
+               simp: readRefillNext_def refillNext_def readSchedContext_def getObject_def[symmetric]
+                     getSchedContext_def[symmetric])
+   apply (rule ccorres_pre_getObject_sc, rename_tac sc)
+   apply (rule ccorres_move_c_guard_sc)
+   apply (rule ccorres_return_C; clarsimp)
+  apply (rule conjI)
+   apply clarsimp
+  apply (clarsimp simp: active_sc_at'_def)
+  apply normalise_obj_at'
+  apply (rename_tac sc' sc)
+  apply (frule (1) obj_at_cslift_sc)
+  apply (clarsimp simp: typ_heap_simps csched_context_relation_def split: if_splits)
+  apply (prop_tac "0 < scRefillMax sc")
+   apply (clarsimp simp: active_sc_at'_def obj_at'_def)
+  apply (frule (1) invs'_ko_at_valid_sched_context')
+  apply (clarsimp simp: word_bits_def)
+  apply (frule (1) length_scRefills_bounded)
+  apply (intro conjI impI allI)
+   apply (cut_tac x=idx
+              and y="unat (scRefillMax_C sc') - Suc 0"
+              and 'a1=machine_word_len
+               in inj_on_contraD[OF inj_on_word_of_nat])
+      apply assumption
+     apply fastforce
+    apply (fastforce simp: valid_sched_context'_def word_bits_def)
+   apply fastforce
+  apply (fastforce simp: unat_of_nat_eq unat_add_lem')
+  done
+
+lemma getRefillSize_exs_valid[wp]:
+  "\<lbrace>(=) s\<rbrace> getRefillSize scPtr \<lbrace>\<lambda>r. (=) s\<rbrace>"
+  by (wpsimp simp: getRefillSize_def)
+
+crunch (empty_fail) empty_fail[wp]: getRefillSize
+
+lemma refill_add_tail_ccorres:
+  "ccorres dc xfdc
+     (active_sc_at' scPtr and invs')
+     (\<lbrace>\<acute>sc = Ptr scPtr\<rbrace> \<inter> {s'. crefill_relation new (refill_' s')}) []
+     (refillAddTail scPtr new) (Call refill_add_tail_'proc)"
+  supply sched_context_C_size[simp del] refill_C_size[simp del] len_bit0[simp del]
+
+  apply (simp add: refillAddTail_def)
+  apply (rule ccorres_symb_exec_l'[rotated, OF _ getRefillSize_sp]; wpsimp)
+  apply (rule ccorres_symb_exec_l'[rotated, OF _ get_sc_sp']; wpsimp?)
+  apply (rule ccorres_symb_exec_l'[rotated, OF _ assert_sp]; wpsimp)
+
+  apply (cinit' lift: sc_' refill_' simp: updateRefillIndex_def)
+   apply (rule ccorres_move_c_guard_sc)
+   apply (ctac add: refill_next_ccorres)
+     apply (rule ccorres_move_c_guard_sc)
+     apply clarsimp
+     apply (rule ccorres_split_nothrow[where r'=dc and xf'=xfdc])
+         apply (rule_tac P=\<top> in updateSchedContext_ccorres_lemma2)
+           apply vcg
+          apply fastforce
+         apply clarsimp
+         apply (rule_tac sc'="scRefillTail_C_update (\<lambda>_. new_tail) sc'"
+                      in rf_sr_sc_update_no_refill_buffer_update2;
+                fastforce?)
+           apply (clarsimp simp: typ_heap_simps')
+          apply (clarsimp simp: csched_context_relation_def)
+         apply (fastforce intro: refill_buffer_relation_sc_no_refills_update)
+        apply ceqv
+       apply (rule_tac P="\<lambda>sc. scRefillTail sc = unat new_tail"
+                   and P'="active_sc_at' scPtr and invs'"
+                    in updateSchedContext_ccorres_lemma3)
+         apply vcg
+        apply fastforce
+       apply normalise_obj_at'
+       apply (frule (1) sc_ko_at_valid_objs_valid_sc'[OF _ invs_valid_objs'])
+       apply (intro conjI)
+          apply (fastforce dest: sc_at_h_t_valid[rotated])
+         apply (rule disjCI2)
+         apply (rule_tac n="length (scRefills sc)" in array_assertion_shrink_right)
+          apply (fastforce intro: sc_at_array_assertion'
+                            simp: valid_sched_context'_def MIN_REFILLS_def)
+         apply (clarsimp simp: typ_heap_simps valid_sched_context'_def obj_at_simps
+                               active_sc_at'_def csched_context_relation_def)
+        apply (frule rf_sr_refill_buffer_relation)
+        apply (frule_tac n="scRefillTail sc" in h_t_valid_refill; fastforce?)
+          apply (clarsimp simp: valid_sched_context'_def active_sc_at'_def obj_at'_def)
+         apply fastforce
+        apply (clarsimp simp: sc_ptr_to_crefill_ptr_def typ_heap_simps csched_context_relation_def)
+       apply (clarsimp simp: ret__ptr_to_struct_refill_C_'_update_rf_sr_helper
+                       cong: StateSpace.state.fold_congs)
+       apply (rule_tac old_sc=sc and n="scRefillTail sc" and refill=new and refill'=refill
+                    in rf_sr_refill_update2;
+              fastforce?)
+          apply (clarsimp simp: valid_sched_context'_def active_sc_at'_def obj_at'_def)
+         apply (fastforce simp: sched_context.expand)
+        apply (clarsimp simp: typ_heap_simps sc_ptr_to_crefill_ptr_def csched_context_relation_def)
+       apply (clarsimp simp: csched_context_relation_def)
+      apply ((rule hoare_vcg_conj_lift
+              | wpsimp wp: updateSchedContext_active_sc_at' updateSchedContext_refills_invs'
+              | wpsimp wp: updateSchedContext_wp)+)[1]
+     apply vcg
+    apply (wpsimp wp: getRefillNext_wp)
+   apply vcg
+  apply normalise_obj_at'
+  apply (frule (1) sc_ko_at_valid_objs_valid_sc'[OF _ invs_valid_objs'])
+  apply (elim conjE)
+  apply (frule (1) length_scRefills_bounded)
+  apply (intro conjI)
+      apply (clarsimp simp: valid_sched_context'_def word_bits_len_of refillSizeBytes_def)
+     apply (fastforce simp: obj_at'_def objBits_simps opt_map_def ps_clear_def)
+    apply (fastforce simp: valid_sched_context'_def refillNext_def refillSize_def split: if_splits)
+   apply (clarsimp simp: valid_sched_context_size'_def)
+  apply (fastforce dest: obj_at_cslift_sc simp: csched_context_relation_def typ_heap_simps)
+  done
+
+lemma maybe_add_empty_tail_ccorres:
+  "ccorres dc xfdc
+     (active_sc_at' scPtr and invs') \<lbrace>\<acute>sc = Ptr scPtr\<rbrace> []
+     (maybeAddEmptyTail scPtr) (Call maybe_add_empty_tail_'proc)"
+  apply (cinit lift: sc_')
+   apply (ctac add: isRoundRobin_ccorres)
+     apply (clarsimp simp: when_def)
+     apply (rule ccorres_cond[where R=\<top>])
+       apply (clarsimp simp: to_bool_def)
+      apply (rule ccorres_rhs_assoc)
+      apply (rule_tac xf'="\<lambda>s. h_val (hrs_mem (t_hrs_' (globals s)))
+                                     (ret__ptr_to_struct_refill_C_' s)"
+                   in ccorres_split_nothrow)
+          apply (rule ccorres_call)
+             apply (rule refill_head_ccorres, clarsimp+)
+         apply ceqv
+        apply (rule ccorres_Guard_Seq)
+        apply (rule ccorres_symb_exec_r)
+          apply (ctac add: refill_add_tail_ccorres)
+         apply vcg
+        apply (rule conseqPre, vcg)
+        apply clarsimp
+       apply (wpsimp wp: getRefillHead_wp)
+      apply vcg
+     apply (rule ccorres_return_Skip')
+    apply (wpsimp wp: isRoundRobin_wp)
+   apply (vcg exspec=isRoundRobin_modifies)
+  apply (rule conjI)
+   apply fastforce
+  apply (clarsimp simp: active_sc_at'_rewrite)
+  apply (frule (1) obj_at_cslift_sc)
+  apply normalise_obj_at'
+  apply (rename_tac sc sc')
+  apply (frule (1) invs'_ko_at_valid_sched_context')
+  apply (frule rf_sr_refill_buffer_relation)
+  apply (frule_tac n="scRefillHead sc" and scPtr=scPtr in h_t_valid_refill; fastforce?)
+   apply (clarsimp simp: valid_sched_context'_def obj_at'_def is_active_sc'_def in_omonad)
+  apply (clarsimp simp: h_val_field_from_bytes' crefill_relation_def typ_heap_simps
+                        sc_ptr_to_crefill_ptr_def csched_context_relation_def)
+  done
+
+lemma maxRefills_helper:
+  "obj_at' (\<lambda>sc :: sched_context. maxRefills \<le> refillAbsoluteMax' (objBits sc)) scPtr s
+   \<Longrightarrow> maxRefills < 2 ^ LENGTH(64)"
+  supply len_bit0[simp del]
+  apply normalise_obj_at'
+  apply (rename_tac sc)
+  apply (rule_tac y="refillAbsoluteMax' (objBits sc)" in le_less_trans)
+   apply fastforce
+  apply (clarsimp simp: obj_at'_def)
+  apply (cut_tac n="objBits sc" in refillAbsoluteMax'_leq)
+   apply (rule_tac y="2 ^ minSchedContextBits" in order_trans)
+    apply (fastforce intro: schedContextStructSize_minSchedContextBits)
+   apply (clarsimp simp: objBits_simps)
+  apply (rule_tac y="2 ^ objBits sc" in le_less_trans)
+   apply (fastforce simp: refillSizeBytes_def)
+  apply (fastforce simp: objBits_simps word_bits_def)
+  done
+
 lemma refill_new_ccorres:
   "ccorres dc xfdc
-     invs'
-     (\<lbrace>\<acute>sc = Ptr scPtr\<rbrace>
-      \<inter> \<lbrace>\<acute>max_refills = of_nat maxRefills\<rbrace>
-      \<inter> \<lbrace>\<acute>budget = budget\<rbrace>
+     (invs'
+      and K (0 < maxRefills)
+      and obj_at' (\<lambda>sc :: sched_context. maxRefills \<le> refillAbsoluteMax' (objBits sc)) scPtr)
+     (\<lbrace>\<acute>sc = Ptr scPtr\<rbrace> \<inter> \<lbrace>\<acute>max_refills = of_nat maxRefills\<rbrace> \<inter> \<lbrace>\<acute>budget = budget\<rbrace>
       \<inter> \<lbrace>\<acute>period = period\<rbrace>) []
      (refillNew scPtr maxRefills budget period) (Call refill_new_'proc)"
-sorry (* FIXME RT: refill_new_ccorres *)
+  (is "ccorres _ _ ?abs _ _ _ _")
+  supply len_bit0[simp del] sched_context_C_size[simp del] refill_C_size[simp del]
+
+  apply (cinit lift: sc_' max_refills_' budget_' period_')
+   apply (rule ccorres_pre_getCurTime, rename_tac curTime)
+  \<comment> \<open>bundle individual updateSchedContext steps updating the scPeriod, scRefillHead, scRefillTail,
+      and scRefillMax into one large updateSchedContext\<close>
+   apply (rule_tac Q5="?abs and (\<lambda>s. ksCurTime s = curTime)"
+                in monadic_rewrite_ccorres_assemble[rotated, where P=Q and Q=Q for Q, simplified],
+          subst bind_assoc[symmetric],
+          rule monadic_rewrite_bind_head,
+          subst bind_dummy_ret_val,
+          rule monadic_rewrite_guard_imp,
+          rule updateSchedContext_decompose[THEN monadic_rewrite_sym],
+          clarsimp simp: objBits_simps active_sc_at'_rewrite)+
+   apply (rule stronger_ccorres_guard_imp[where A'=Q' and Q'=Q' for Q', simplified])
+     apply (rule ccorres_move_c_guard_sc)
+     \<comment> \<open>break off the part of the C corresponding to the bundled updateSchedContext step\<close>
+     apply (rule ccorres_rhs_assoc2)
+     apply (rule ccorres_rhs_assoc2)
+     apply (rule ccorres_rhs_assoc2)
+     apply (rule_tac r'=dc and xf'=xfdc in ccorres_split_nothrow)
+         apply (rule updateSchedContext_ccorres_lemma3
+                      [where P=\<top> and P'="K (maxRefills < 2 ^ LENGTH(64))"])
+           apply (vcg exspec=refill_index_modifies)
+          apply fastforce
+         apply clarsimp
+         apply (rule conjI)
+          apply (fastforce dest: obj_at_cslift_sc simp: typ_heap_simps')
+         apply (rule rf_sr_sc_update_no_refill_buffer_update2; fastforce?)
+           apply (fastforce simp: typ_heap_simps' packed_heap_update_collapse_hrs)
+          apply (clarsimp simp: csched_context_relation_def)
+          apply (subst unat_of_nat_eq)
+           apply (simp add: word_bits_def)
+          apply (rule refl)
+         apply (fastforce intro: refill_buffer_relation_sc_no_refills_update)
+        apply ceqv
+       apply (rule ccorres_rhs_assoc2)
+       apply (rule ccorres_split_nothrow)
+           apply (clarsimp simp: setRefillHd_def updateRefillHd_def)
+           apply (rule_tac P'="invs' and (\<lambda>s. ksCurTime s = curTime)"
+                        in updateSchedContext_ccorres_lemma3
+                            [where P="\<lambda>sc. scRefillHead sc < length (scRefills sc)"])
+             apply (vcg expsec=refill_head_modifies )
+            apply fastforce
+           apply clarsimp
+           apply (rename_tac sc sc')
+           apply (frule (1) obj_at_cslift_sc)
+           apply (frule (1) sc_ko_at_valid_objs_valid_sc'[OF _ invs_valid_objs'])
+           apply (frule rf_sr_refill_buffer_relation)
+           apply (intro conjI)
+              apply (clarsimp simp: typ_heap_simps)
+             apply (rule disjCI2)
+             apply (rule_tac n="length (scRefills sc)" in array_assertion_shrink_right)
+              apply (rule sc_at_array_assertion'; assumption?)
+              apply (clarsimp simp: valid_sched_context'_def MIN_REFILLS_def)
+             apply (clarsimp simp: typ_heap_simps csched_context_relation_def)
+            apply (frule_tac n=0 in h_t_valid_refill; fastforce?)
+              apply clarsimp
+             apply fastforce
+            apply (clarsimp simp: sc_ptr_to_crefill_ptr_def typ_heap_simps)
+            apply (frule_tac n="scRefillHead sc" in h_t_valid_refill; fastforce?)
+             apply fastforce
+            apply (clarsimp simp: sc_ptr_to_crefill_ptr_def csched_context_relation_def)
+           apply (clarsimp simp: ret__ptr_to_struct_refill_C_'_update_rf_sr_helper
+                           cong: StateSpace.state.fold_congs)
+           apply (rule_tac old_sc=sc and n="scRefillHead sc"
+                       and fa="\<lambda>refill. rAmount_update (\<lambda>_. budget) refill"
+                        in rf_sr_refill_update2;
+                  fastforce?)
+              apply (fastforce simp: sched_context.expand)
+             apply (frule_tac n="scRefillHead sc" in h_t_valid_refill; fastforce?)
+              apply fastforce
+             apply (clarsimp simp: valid_sched_context'_def)
+             apply (fastforce simp: typ_heap_simps sc_ptr_to_crefill_ptr_def
+                                    csched_context_relation_def)
+            apply (clarsimp simp: csched_context_relation_def)
+           apply (drule_tac n="scRefillHead sc" in crefill_relationD; fastforce?)
+           apply (fastforce simp: crefill_relation_def sc_ptr_to_crefill_ptr_def
+                                  csched_context_relation_def)
+          apply ceqv
+         apply (rule ccorres_rhs_assoc2)
+         apply (rule ccorres_split_nothrow)
+             apply (clarsimp simp: setRefillHd_def updateRefillHd_def)
+             apply (rule_tac P'="invs' and (\<lambda>s. ksCurTime s = curTime)"
+                          in updateSchedContext_ccorres_lemma3
+                              [where P="\<lambda>sc. scRefillHead sc < length (scRefills sc)"])
+               apply (vcg expsec=refill_head_modifies)
+              apply fastforce
+             apply normalise_obj_at'
+             apply (rename_tac sc sc')
+             apply (frule (1) obj_at_cslift_sc)
+             apply (frule (1) sc_ko_at_valid_objs_valid_sc'[OF _ invs_valid_objs'])
+             apply (frule rf_sr_refill_buffer_relation)
+             apply (intro conjI impI allI)
+                apply (clarsimp simp: ptr_add_assertion_def typ_heap_simps)
+               apply (rule disjCI2)
+               apply (rule_tac n="length (scRefills sc)" in array_assertion_shrink_right)
+                apply (rule sc_at_array_assertion'; assumption?)
+                apply (clarsimp simp: valid_sched_context'_def MIN_REFILLS_def)
+               apply (clarsimp simp: typ_heap_simps csched_context_relation_def)
+              apply (frule_tac n=0 in h_t_valid_refill; fastforce?)
+                apply clarsimp
+               apply fastforce
+              apply (clarsimp simp: sc_ptr_to_crefill_ptr_def typ_heap_simps)
+              apply (frule_tac n="scRefillHead sc" in h_t_valid_refill; fastforce?)
+               apply fastforce
+              apply (clarsimp simp: sc_ptr_to_crefill_ptr_def csched_context_relation_def)
+             apply (clarsimp simp: ret__ptr_to_struct_refill_C_'_update_rf_sr_helper
+                             cong: StateSpace.state.fold_congs)
+             apply (rule_tac old_sc=sc and n="scRefillHead sc"
+                         and fa="\<lambda>refill. rTime_update (\<lambda>_. ksCurTime s) refill"
+                          in rf_sr_refill_update2;
+                    fastforce?)
+                apply (fastforce simp: sched_context.expand)
+               apply (frule_tac n="scRefillHead sc" in h_t_valid_refill; fastforce?)
+                apply fastforce
+               apply (clarsimp simp: valid_sched_context'_def)
+               apply (fastforce simp: typ_heap_simps sc_ptr_to_crefill_ptr_def
+                                      csched_context_relation_def)
+              apply (clarsimp simp: csched_context_relation_def)
+             apply (drule_tac n="scRefillHead sc" in crefill_relationD; fastforce?)
+             apply (clarsimp simp: crefill_relation_def sc_ptr_to_crefill_ptr_def
+                                   csched_context_relation_def
+                            dest!: rf_sr_ksCurTime)
+            apply ceqv
+           apply (ctac add: maybe_add_empty_tail_ccorres)
+          apply (wpsimp wp: updateRefillHd_invs')
+         apply (vcg exspec=refill_head_modifies)
+        apply ((rule hoare_vcg_conj_lift
+                | wpsimp wp: updateRefillHd_invs'
+                | wpsimp simp: updateRefillHd_def wp: updateSchedContext_wp)+)[1]
+       apply (vcg exspec=refill_head_modifies)
+      apply (rule_tac Q="\<lambda>_ s. active_sc_at' scPtr s \<and> invs' s \<and> ksCurTime s = curTime
+                               \<and> obj_at' (\<lambda>sc. scRefillHead sc < length (scRefills sc)) scPtr s"
+                   in hoare_post_imp)
+       apply (fastforce simp: obj_at'_def objBits_simps opt_map_def ps_clear_def)
+      apply ((rule hoare_vcg_conj_lift
+              | wpsimp wp: updateSchedContext_refills_invs'
+              | wpsimp simp: updateRefillHd_def
+                         wp: updateSchedContext_wp)+)[1]
+     apply vcg
+    defer
+    apply fastforce
+   apply fastforce
+  apply clarsimp
+  apply (frule maxRefills_helper)
+  apply normalise_obj_at'
+  apply (frule (1) invs'_ko_at_valid_sched_context')
+  apply (fastforce simp: obj_at'_def valid_sched_context'_def opt_map_def active_sc_at'_def
+                         refillSize_def objBits_simps ps_clear_def)
+  done
 
 lemma refill_update_ccorres:
   "ccorres dc xfdc
-     invs'
-     (\<lbrace>\<acute>sc = Ptr scPtr\<rbrace>
-      \<inter> \<lbrace>\<acute>new_period = newPeriod\<rbrace>
-      \<inter> \<lbrace>\<acute>new_budget = newBudget\<rbrace>
+     (active_sc_at' scPtr and invs'
+      and K (0 < newMaxRefills)
+      and obj_at' (\<lambda>sc :: sched_context. newMaxRefills \<le> refillAbsoluteMax' (objBits sc)) scPtr)
+     (\<lbrace>\<acute>sc = Ptr scPtr\<rbrace> \<inter> \<lbrace>\<acute>new_period = newPeriod\<rbrace> \<inter> \<lbrace>\<acute>new_budget = newBudget\<rbrace>
       \<inter> \<lbrace>\<acute>new_max_refills = of_nat newMaxRefills\<rbrace>) []
      (refillUpdate scPtr newPeriod newBudget newMaxRefills) (Call refill_update_'proc)"
-sorry (* FIXME RT: refill_update_ccorres *)
+  supply len_bit0[simp del] sched_context_C_size[simp del] refill_C_size[simp del]
+
+  apply (cinit lift: sc_' new_period_' new_budget_' new_max_refills_')
+   \<comment> \<open>break off the part of the C corresponding to update to the scRefills field\<close>
+   apply (rule ccorres_rhs_assoc2)
+   apply (rule ccorres_rhs_assoc2)
+   apply (rule_tac r'=dc and xf'=xfdc in ccorres_split_nothrow)
+       apply (rule updateSchedContext_ccorres_lemma3
+                   [where P=\<top> and P'="invs' and active_sc_at' scPtr"])
+         apply (vcg expsec=refill_index_modifies)
+        apply fastforce
+       apply normalise_obj_at'
+       apply (rename_tac sc sc')
+       apply (frule (1) obj_at_cslift_sc)
+       apply (frule (1) sc_ko_at_valid_objs_valid_sc'[OF _ invs_valid_objs'])
+       apply (frule rf_sr_refill_buffer_relation)
+       apply (intro conjI)
+            apply (clarsimp simp: ptr_add_assertion_def)
+           apply (clarsimp simp: typ_heap_simps)
+          apply (rule disjCI2)
+          apply (rule_tac n="length (scRefills sc)" in array_assertion_shrink_right)
+           apply (fastforce intro: sc_at_array_assertion'
+                             simp: valid_sched_context'_def MIN_REFILLS_def)
+          apply (clarsimp simp: typ_heap_simps valid_sched_context'_def obj_at'_def
+                                active_sc_at'_def csched_context_relation_def)
+         apply (frule_tac n=0 in h_t_valid_refill; fastforce?)
+           apply (clarsimp simp: csched_context_relation_def valid_sched_context'_def
+                                 active_sc_at'_def obj_at'_def)
+          apply fastforce
+         apply (clarsimp simp: sc_ptr_to_crefill_ptr_def typ_heap_simps)
+        apply (frule_tac n="scRefillHead sc" in h_t_valid_refill; fastforce?)
+          apply (clarsimp simp: csched_context_relation_def valid_sched_context'_def
+                                active_sc_at'_def obj_at'_def)
+         apply fastforce
+        apply (clarsimp simp: sc_ptr_to_crefill_ptr_def csched_context_relation_def
+                              typ_heap_simps)
+       apply (clarsimp simp: ret__ptr_to_struct_refill_C_'_update_rf_sr_helper
+                       cong: StateSpace.state.fold_congs)
+       apply (rule_tac n=0 and fa="\<lambda>_. refillHd sc" in rf_sr_refill_update2; fastforce?)
+           apply (clarsimp simp: valid_sched_context'_def MIN_REFILLS_def)
+          apply (fastforce simp: sched_context.expand)
+         apply (fastforce simp: typ_heap_simps' sc_ptr_to_crefill_ptr_def)
+        apply (clarsimp simp: csched_context_relation_def)
+       apply (drule_tac n="scRefillHead sc" in crefill_relationD; fastforce?)
+        apply (clarsimp simp: csched_context_relation_def valid_sched_context'_def
+                              active_sc_at'_def obj_at'_def)
+       apply (clarsimp simp: sc_ptr_to_crefill_ptr_def refillHd_def csched_context_relation_def)
+      apply ceqv
+
+     \<comment> \<open>bundle all updates to the sched context into one updateSchedContext step\<close>
+     apply (rule monadic_rewrite_ccorres_assemble[rotated], clarsimp,
+            subst bind_assoc[symmetric],
+            rule monadic_rewrite_bind_head, subst bind_dummy_ret_val,
+            rule monadic_rewrite_guard_imp,
+            rule updateSchedContext_decompose[THEN monadic_rewrite_sym],
+            clarsimp simp: objBits_simps active_sc_at'_rewrite, assumption)+
+     apply (rule ccorres_rhs_assoc2)
+     apply (rule ccorres_rhs_assoc2)
+     apply (rule ccorres_rhs_assoc2)
+     apply (rule_tac r'=dc and xf'=xfdc in ccorres_split_nothrow)
+         \<comment> \<open>show correspondence between the updates to the sched context struct fields\<close>
+         apply clarsimp
+         apply (rule updateSchedContext_ccorres_lemma2[where P="K (newMaxRefills < 2 ^ word_bits)"])
+           apply vcg
+          apply fastforce
+         apply (clarsimp simp: typ_heap_simps)
+         apply (rule_tac sc'="scRefillTail_C_update (\<lambda>_. 0)
+                               (scRefillHead_C_update (\<lambda>_. 0)
+                                (scRefillMax_C_update (\<lambda>_. word_of_nat newMaxRefills)
+                                 (scPeriod_C_update (\<lambda>_. newPeriod) sc')))"
+                      in rf_sr_sc_update_no_refill_buffer_update2;
+                fastforce?)
+           apply (clarsimp simp: typ_heap_simps' packed_heap_update_collapse_hrs)
+          apply (fastforce simp: csched_context_relation_def unat_of_nat_eq word_bits_def)
+         apply (fastforce intro: refill_buffer_relation_sc_no_refills_update)
+        apply ceqv
+
+       apply (clarsimp simp: whenM_def ifM_def bind_assoc)
+       apply (ctac add: refill_ready_ccorres)
+         apply (rule_tac r'=dc and xf'=xfdc in ccorres_split_nothrow)
+             apply (rule ccorres_cond[where R=\<top>])
+               apply (clarsimp simp: to_bool_def)
+              apply (rule ccorres_pre_getCurTime, rename_tac curTime)
+              apply (clarsimp simp: updateRefillHd_def)
+              apply (rule_tac P=\<top>
+                          and P'="\<lambda>s. ksCurTime s = curTime \<and> invs' s \<and> active_sc_at' scPtr s"
+                          and Q="\<lambda>s sc. {s'. (s, s') \<in> rf_sr \<and> ko_at' sc scPtr s \<and> invs' s
+                                             \<and> active_sc_at' scPtr s \<and> ksCurTime s = curTime}"
+                           in updateSchedContext_ccorres_lemma3)
+                apply (rule conseqPre, vcg)
+                apply normalise_obj_at'
+                apply (rename_tac sc sc')
+                apply (frule (1) obj_at_cslift_sc)
+                apply clarsimp
+                apply (frule (1) sc_ko_at_valid_objs_valid_sc'[OF _ invs_valid_objs'])
+                apply (frule rf_sr_refill_buffer_relation)
+                apply (intro conjI)
+                   apply (clarsimp simp: typ_heap_simps)
+                  apply (rule disjCI2)
+                  apply (rule_tac n="length (scRefills sc)" in array_assertion_shrink_right)
+                   apply (fastforce intro: sc_at_array_assertion'
+                                     simp: valid_sched_context'_def MIN_REFILLS_def)
+                  apply (clarsimp simp: typ_heap_simps valid_sched_context'_def obj_at'_def
+                                        active_sc_at'_def csched_context_relation_def)
+                 apply (frule_tac n="scRefillHead sc" in h_t_valid_refill; fastforce?)
+                   apply (clarsimp simp: csched_context_relation_def valid_sched_context'_def
+                                         active_sc_at'_def obj_at'_def)
+                  apply fastforce
+                 apply (clarsimp simp: sc_ptr_to_crefill_ptr_def csched_context_relation_def
+                                       typ_heap_simps)
+                apply (clarsimp simp: ret__ptr_to_struct_refill_C_'_update_rf_sr_helper
+                                cong: StateSpace.state.fold_congs)
+                apply (rule_tac old_sc=sc and n="scRefillHead sc"
+                                and fa="\<lambda>refill. rTime_update (\<lambda>_. ksCurTime s) refill"
+                                 in rf_sr_refill_update2;
+                       fastforce?)
+                    apply (clarsimp simp: valid_sched_context'_def active_sc_at'_def obj_at'_def)
+                   apply (fastforce simp: sched_context.expand)
+                  apply (frule_tac n="scRefillHead sc" in h_t_valid_refill; fastforce?)
+                    apply (clarsimp simp: valid_sched_context'_def active_sc_at'_def obj_at'_def)
+                   apply fastforce
+                  apply (clarsimp simp: valid_sched_context'_def)
+                  apply (fastforce simp: h_val_field_from_bytes' typ_heap_simps
+                                         sc_ptr_to_crefill_ptr_def csched_context_relation_def)
+                 apply (clarsimp simp: csched_context_relation_def)
+                apply (drule_tac n="scRefillHead sc" in crefill_relationD; fastforce?)
+                 apply (clarsimp simp: valid_sched_context'_def active_sc_at'_def obj_at'_def
+                                       csched_context_relation_def)
+                apply (fastforce simp: crefill_relation_def sc_ptr_to_crefill_ptr_def
+                                       csched_context_relation_def
+                                 dest: rf_sr_ksCurTime)
+               apply fastforce
+              apply clarsimp
+             apply (rule ccorres_return_Skip')
+            apply ceqv
+
+           apply (rule_tac xf'="\<lambda>s. h_val (hrs_mem (t_hrs_' (globals s)))
+                                          (ret__ptr_to_struct_refill_C_' s)"
+                        in ccorres_split_nothrow)
+               apply (rule ccorres_call)
+                  apply (rule refill_head_ccorres, clarsimp+)
+              apply ceqv
+             apply (rename_tac refill refill')
+             apply (rule ccorres_Guard)
+             apply (rule_tac R="sc_at' scPtr"
+                         and R'="\<lbrace>h_val (hrs_mem \<acute>t_hrs) \<acute>ret__ptr_to_struct_refill_C = refill'\<rbrace>"
+                         and Pt="invs' and active_sc_at' scPtr"
+                         and Pf="invs' and active_sc_at' scPtr
+                                 and (obj_at' (\<lambda>sc. refillHd sc = refill) scPtr)"
+                         and Rt=UNIV
+                         and Rf="\<lbrace>h_val (hrs_mem \<acute>t_hrs) \<acute>ret__ptr_to_struct_refill_C = refill'\<rbrace>"
+                          in ccorres_cond_strong)
+               apply (clarsimp simp: h_val_field_from_bytes' crefill_relation_def)
+
+              \<comment> \<open>newBudget \<le> rAmount refill - update the rAmount and perform maybeAddEmptyTail\<close>
+              apply (rule stronger_ccorres_guard_imp)
+                apply (rule_tac r'=dc and xf'=xfdc in ccorres_split_nothrow)
+                    apply (clarsimp simp: updateRefillHd_def)
+                    apply (rule_tac P=\<top> and P'="\<lambda>s. invs' s \<and> active_sc_at' scPtr s"
+                                and Q="\<lambda>s sc. {s'. (s, s') \<in> rf_sr \<and> ko_at' sc scPtr s \<and> invs' s
+                                                   \<and> active_sc_at' scPtr s}"
+                                 in updateSchedContext_ccorres_lemma3)
+                      apply (rule conseqPre, vcg)
+                      apply normalise_obj_at'
+                      apply (rename_tac sc sc')
+                      apply (frule (1) obj_at_cslift_sc)
+                      apply (frule (1) sc_ko_at_valid_objs_valid_sc'[OF _ invs_valid_objs'])
+                      apply (frule rf_sr_refill_buffer_relation)
+                      apply (intro conjI impI allI)
+                         apply (clarsimp simp: typ_heap_simps)
+                        apply (rule disjCI2)
+                        apply (rule_tac n="length (scRefills sc)" in array_assertion_shrink_right)
+                         apply (fastforce intro: sc_at_array_assertion'
+                                           simp: valid_sched_context'_def MIN_REFILLS_def)
+                        apply (clarsimp simp: typ_heap_simps valid_sched_context'_def obj_at'_def
+                                              active_sc_at'_def csched_context_relation_def)
+                       apply (frule_tac n="scRefillHead sc" in h_t_valid_refill; fastforce?)
+                         apply (clarsimp simp: csched_context_relation_def valid_sched_context'_def
+                                               active_sc_at'_def obj_at'_def)
+                        apply fastforce
+                       apply (clarsimp simp: sc_ptr_to_crefill_ptr_def csched_context_relation_def
+                                             typ_heap_simps)
+                      apply (clarsimp simp: ret__ptr_to_struct_refill_C_'_update_rf_sr_helper
+                                      cong: StateSpace.state.fold_congs)
+                      apply (rule_tac old_sc=sc and n="scRefillHead sc"
+                                  and fa="\<lambda>refill. rAmount_update (\<lambda>_. newBudget) refill"
+                                   in rf_sr_refill_update2)
+                                apply fastforce
+                               apply fastforce
+                              apply fastforce
+                             apply fastforce
+                            apply (clarsimp simp: valid_sched_context'_def active_sc_at'_def
+                                                  obj_at'_def)
+                           apply (fastforce simp: sched_context.expand)
+                          apply fastforce
+                         apply (frule_tac n="scRefillHead sc" in h_t_valid_refill; fastforce?)
+                           apply (clarsimp simp: valid_sched_context'_def active_sc_at'_def
+                                                 obj_at'_def)
+                          apply fastforce
+                         apply (clarsimp simp: valid_sched_context'_def)
+                         apply (fastforce simp: typ_heap_simps sc_ptr_to_crefill_ptr_def
+                                                csched_context_relation_def)
+                        apply (fastforce simp: csched_context_relation_def)
+                       apply (rule refl)
+                      apply (drule_tac n="scRefillHead sc" in crefill_relationD; fastforce?)
+                       apply (clarsimp simp: csched_context_relation_def valid_sched_context'_def
+                                             active_sc_at'_def obj_at'_def)
+                      apply (fastforce simp: crefill_relation_def sc_ptr_to_crefill_ptr_def
+                                             csched_context_relation_def)
+                     apply fastforce
+                    apply fastforce
+                   apply ceqv
+                  apply clarsimp
+                  apply (ctac add: maybe_add_empty_tail_ccorres)
+                 apply (wpsimp wp: updateRefillHd_invs')
+                apply vcg
+               apply (clarsimp simp: active_sc_at'_rewrite)
+              apply clarsimp
+
+             \<comment> \<open>rAmount refill < newBudget - perform refillAddTail\<close>
+             apply (rule stronger_ccorres_guard_imp)
+               apply clarsimp
+               apply (rule ccorres_rhs_assoc)+
+               apply (rule ccorres_symb_exec_r)
+                 apply (rule ccorres_symb_exec_r)
+                   apply (rule ccorres_Guard_Seq)+
+                   apply (rule ccorres_symb_exec_r)
+                     apply (ctac add: refill_add_tail_ccorres)
+                    apply vcg
+                   apply (rule conseqPre, vcg)
+                   apply clarsimp
+                  apply vcg
+                 apply (rule conseqPre, vcg)
+                 apply clarsimp
+                apply vcg
+               apply (rule conseqPre, vcg)
+               apply clarsimp
+              apply wpsimp
+             apply wpsimp
+             apply (clarsimp cong: conj_cong)
+             apply normalise_obj_at'
+             apply (rename_tac sc)
+             apply (frule (1) obj_at_cslift_sc)
+             apply (frule (1) sc_ko_at_valid_objs_valid_sc'[OF _ invs_valid_objs'])
+             apply (frule rf_sr_refill_buffer_relation)
+             apply (frule_tac n="scRefillHead sc" in h_t_valid_refill; fastforce?)
+               apply (fastforce simp: valid_sched_context'_def obj_at_simps active_sc_at'_def)
+              apply fastforce
+             apply (intro conjI impI allI)
+                apply (clarsimp simp: typ_heap_simps)
+               apply (rule disjCI2)
+               apply (rule_tac n="length (scRefills sc)" in array_assertion_shrink_right)
+                apply (fastforce intro: sc_at_array_assertion'
+                                  simp: valid_sched_context'_def MIN_REFILLS_def)
+               apply (fastforce simp: typ_heap_simps valid_sched_context'_def obj_at_simps
+                                      active_sc_at'_def csched_context_relation_def)
+              apply (frule_tac n="scRefillHead sc" in crefill_relationD; fastforce?)
+               apply (clarsimp simp: valid_sched_context'_def active_sc_at'_def obj_at'_def)
+              apply (clarsimp simp: h_val_field_from_bytes' sc_ptr_to_crefill_ptr_def typ_heap_simps
+                                    crefill_relation_def csched_context_relation_def refillHd_def)
+             apply (clarsimp simp: sc_ptr_to_crefill_ptr_def csched_context_relation_def
+                                   typ_heap_simps)
+            apply (rule_tac Q="\<lambda>refill s. (invs' s \<and> active_sc_at' scPtr s)
+                                          \<and> obj_at' (\<lambda>sc. refillHd sc = refill) scPtr s"
+                         in hoare_post_imp)
+             apply fastforce
+            apply (rule getRefillHead_sp)
+           apply vcg
+          apply ((wpsimp wp: updateRefillHd_invs' | strengthen invs_valid_objs')+)[1]
+         apply (vcg exspec=refill_index_modifies)
+        apply (rule_tac Q="\<lambda>_. active_sc_at' scPtr and invs'" in hoare_post_imp)
+         apply (clarsimp simp: active_sc_at'_rewrite)
+        apply (wpsimp wp: refillReady_inv)
+       apply (vcg exspec=refill_ready_modifies)
+      apply (wpsimp wp: updateSchedContext_refills_invs' updateSchedContext_active_sc_at')
+     apply (vcg exspec=refill_index_modifies)
+    apply (rule_tac Q="\<lambda>_ s. invs' s \<and> active_sc_at' scPtr s \<and> 0 < newMaxRefills
+                             \<and> obj_at' (\<lambda>sc. newMaxRefills \<le> refillAbsoluteMax' (objBits sc)) scPtr s"
+                 in hoare_post_imp)
+     apply (clarsimp simp: active_sc_at'_def)
+     apply normalise_obj_at'
+     apply (frule maxRefills_helper)
+     apply (frule (1) sc_ko_at_valid_objs_valid_sc'[OF _ invs_valid_objs'])
+     apply (clarsimp simp: valid_sched_context'_def refillSize_def objBits_simps word_bits_def
+                           obj_at'_def)
+    apply (wpsimp wp: updateSchedContext_refills_invs' updateSchedContext_active_sc_at'
+                      updateSchedContext_wp)
+   apply (vcg exspec=refill_index_modifies)
+  apply normalise_obj_at'
+  apply (rename_tac sc)
+  apply (frule (1) obj_at_cslift_sc)
+  apply (frule (1) sc_ko_at_valid_objs_valid_sc'[OF _ invs_valid_objs'])
+  apply (frule rf_sr_refill_buffer_relation)
+  apply (frule_tac n=0 in h_t_valid_refill; fastforce?)
+    apply (clarsimp simp: valid_sched_context'_def MIN_REFILLS_def)
+   apply fastforce
+  apply (frule_tac n="scRefillHead sc" in h_t_valid_refill; fastforce?)
+    apply (clarsimp simp: valid_sched_context'_def MIN_REFILLS_def obj_at'_def active_sc_at'_def)
+   apply fastforce
+  apply (clarsimp simp: valid_sched_context'_def refillSize_def objBits_simps word_bits_def)
+  apply (rule conjI)
+   apply (clarsimp split: if_splits)
+  apply (rule conjI)
+   apply (fastforce simp: objBits_simps obj_at'_def opt_map_def ps_clear_def)
+  by (clarsimp simp: typ_heap_simps sc_ptr_to_crefill_ptr_def) (* takes ~ 1 minute *)
 
 lemma decodeSchedContext_UnbindObject_ccorres:
   "ccorres dc xfdc
