proof/crefine/RISCV64/Tcb_C.thy
@@ -1151,6 +1151,7 @@ lemma tcbReleaseEnqueue_tcbDomain[wp]:
 
 crunches schedContextResume
   for tcbDomain[wp]: "obj_at' (\<lambda>tcb. P (tcbDomain tcb)) t"
+  (wp: isSchedulable_wp simp: crunch_simps)
 
 lemma schedContextResume_sch_act_wf[wp]:
   "schedContextResume scPtr \<lbrace>\<lambda>s. sch_act_wf (ksSchedulerAction s) s\<rbrace>"
